rupicola/stlc_v2/EquivRel.fsti
@@ -19,8 +19,15 @@ let rec (∋) (t:typsr) (p:get_Type t * closed_exp) : Tot Type0 (decreases %[get
     let fs_f : s1 -> s2 = fs_v in
     match e with
     | ELam e' ->
-      (forall (v:value) (fs_v:s1). (| _, _, r1 |) ∋ (fs_v, v) ==>
-        (| _, _, r2 |) ⦂ (fs_f fs_v, subst_beta v e'))
+      (forall (v:value) (fs_v:s1). (| t1, s1, r1 |) ∋ (fs_v, v) ==>
+        (| t2, s2, r2 |) ⦂ (fs_f fs_v, subst_beta v e'))
+    | _ -> False
+  end
+  | RPair #t1 #t2 #s1 #s2 r1 r2 -> begin
+    let (fs_v1, fs_v2) : s1 * s2 = fs_v in
+    match e with
+    | EPair e1 e2 ->
+      (| t1, s1, r1 |) ∋ (fs_v1, e1) /\ (| t2, s2, r2 |) ∋ (fs_v2, e2)
     | _ -> False
   end
 and (⦂) (t:typsr) (p: get_Type t * closed_exp) : Tot Type0 (decreases %[get_rel t;1]) =
@@ -109,12 +116,16 @@ let equiv_false g
 
 let equiv_var g (x:var{Some? (g x)})
   : Lemma ((fun (fs_s:fs_env g) -> get_v fs_s x) ≈ EVar x)
-  = assert ((fun (fs_s:fs_env g) -> get_v fs_s x) ≈ EVar x) by (explode ())
+  =
+  introduce forall b (s:gsub g b) fs_s. s ∽ fs_s ==>  Some?.v (g x) ⦂ (get_v fs_s x, gsubst s (EVar x)) with begin
+    introduce _ ==> _ with _. begin
+      assert (Some?.v (g x) ∋ (get_v fs_s x, s x));
+      lem_values_are_expressions (Some?.v (g x)) (get_v fs_s x) (s x)
+    end
+  end
 
 let equiv_lam g (t1:typsr) (body:exp) (t2:typsr) (f:fs_env g -> get_Type (mk_arrow t1 t2)) : Lemma
   (requires (fun (fs_s:fs_env (extend t1 g)) -> f (fs_shrink #t1 fs_s) (get_v fs_s 0)) ≈ body)
-            // the asymmetry is here. body is an open expression, while for f, I don't have an open expression
-            // the equiv is quantifying over the free variable of body, but not get_v
   (ensures f ≈ (ELam body)) =
   lem_fv_in_env_lam g t1 body;
   let g' = extend t1 g in
@@ -149,17 +160,27 @@ let equiv_app g (t1:typsr) (t2:typsr) (e1:exp) (e2:exp) (fs_e1:fs_env g -> get_T
   (ensures (fun fs_s -> (fs_e1 fs_s) (fs_e2 fs_s)) ≈ (EApp e1 e2)) =
   lem_fv_in_env_app g e1 e2;
   introduce forall b (s:gsub g b) fs_s. s ∽ fs_s ==> t2 ⦂ ((fs_e1 fs_s) (fs_e2 fs_s), gsubst s (EApp e1 e2)) with begin
-    let fs_e1' = fs_e1 fs_s in
-    let fs_e2' = fs_e2 fs_s in
-    let fs_e = fs_e1' fs_e2' in
-    introduce s ∽ fs_s ==>  t2 ⦂ (fs_e, gsubst s (EApp e1 e2)) with _. begin
-      introduce forall (e':closed_exp). steps (gsubst s (EApp e1 e2)) e' /\ irred e' ==> t2 ∋ (fs_e, e') with begin
+    let fs_e1 = fs_e1 fs_s in
+    let fs_e2 = fs_e2 fs_s in
+    let fs_e = fs_e1 fs_e2 in
+    let e = EApp (gsubst s e1) (gsubst s e2) in
+    assert (gsubst s (EApp e1 e2) == e);
+    let EApp e1 e2 = e in
+    introduce s ∽ fs_s ==>  t2 ⦂ (fs_e, e) with _. begin
+      introduce forall (e':closed_exp). steps e e' /\ irred e' ==> t2 ∋ (fs_e, e') with begin
         introduce _ ==> t2 ∋ (fs_e, e') with h. begin
-          let steps_e_e' : squash (steps (EApp (gsubst s e1) (gsubst s e2)) e') = () in
+          let steps_e_e' : squash (steps e e') = () in
           FStar.Squash.map_squash #_ #(squash (t2 ∋ (fs_e, e'))) steps_e_e' (fun steps_e_e' ->
-            let (e11, e2') = destruct_steps_eapp (gsubst s e1) (gsubst s e2) e' steps_e_e' in
-            assert (mk_arrow t1 t2 ∋ (fs_e1', ELam e11));
-            assert (t1 ∋ (fs_e2', e2'));
+            let (e11, e2') = destruct_steps_eapp e1 e2 e' steps_e_e' in
+            assert (mk_arrow t1 t2 ∋ (fs_e1, ELam e11));
+            introduce True ==>  t1 ∋ (fs_e2, e2') with _. begin
+              assert (t1 ⦂ (fs_e2, e2));
+              assert (steps e2 e2');
+              assert (irred e2')
+            end;
+            eliminate forall (v:value) (fs_v:get_Type t1). t1 ∋ (fs_v, v) ==>
+              t2 ⦂ (fs_e1 fs_v, subst_beta v e11)
+            with e2' fs_e2;
             assert (t2 ⦂ (fs_e, subst_beta e2' e11));
             assert (t2 ∋ (fs_e, e'))
           )
@@ -173,18 +194,47 @@ let equiv_if g (t:typsr) (e1:exp) (e2:exp) (e3:exp) (fs_e1:fs_env g -> get_Type 
   (ensures (fun fs_s -> if fs_e1 fs_s then fs_e2 fs_s else fs_e3 fs_s) ≈ EIf e1 e2 e3) =
   lem_fv_in_env_if g e1 e2 e3;
   introduce forall b (s:gsub g b) fs_s. s ∽ fs_s ==> t ⦂ ((if fs_e1 fs_s then fs_e2 fs_s else fs_e3 fs_s), gsubst s (EIf e1 e2 e3)) with begin
-    let fs_e1' = fs_e1 fs_s in
-    let fs_e2' = fs_e2 fs_s in
-    let fs_e3' = fs_e3 fs_s in
-    let fs_e = if fs_e1' then fs_e2' else fs_e3' in
-    introduce s ∽ fs_s ==>  t ⦂ (fs_e, gsubst s (EIf e1 e2 e3)) with _. begin
-      introduce forall (e':closed_exp). steps (gsubst s (EIf e1 e2 e3)) e' /\ irred e' ==> t ∋ (fs_e, e') with begin
+    let fs_e1 = fs_e1 fs_s in
+    let fs_e = if fs_e1 then fs_e2 fs_s else fs_e3 fs_s in
+    let e = EIf (gsubst s e1) (gsubst s e2) (gsubst s e3) in
+    assert (gsubst s (EIf e1 e2 e3) == e);
+    let EIf e1 e2 e3 = e in
+    introduce s ∽ fs_s ==>  t ⦂ (fs_e, e) with _. begin
+      introduce forall (e':closed_exp). steps e e' /\ irred e' ==> t ∋ (fs_e, e') with begin
         introduce _ ==> t ∋ (fs_e, e') with h. begin
-          let steps_e_e' : squash (steps (EIf (gsubst s e1) (gsubst s e2) (gsubst s e3)) e') = () in
+          let steps_e_e' : squash (steps e e') = () in
           FStar.Squash.map_squash #_ #(squash (t ∋ (fs_e, e'))) steps_e_e' (fun steps_e_e' ->
-            let e1' = destruct_steps_eif (gsubst s e1) (gsubst s e2) (gsubst s e3) e' steps_e_e' in
-            assert (tbool ∋ (fs_e1', e1'));
+            let e1' = destruct_steps_eif e1 e2 e3 e' steps_e_e' in
+            assert (tbool ∋ (fs_e1, e1'));
             assert (t ∋ (fs_e, e'))
+          )
+        end
+      end
+    end
+  end
+
+let equiv_pair g (t1 t2:typsr) (e1:exp) (e2:exp) (fs_e1:fs_env g -> get_Type t1) (fs_e2:fs_env g -> get_Type t2) : Lemma
+  (requires fs_e1 ≈ e1 /\ fs_e2 ≈ e2)
+  (ensures (fun fs_s -> (fs_e1 fs_s, fs_e2 fs_s)) `equiv (mk_pair t1 t2)` EPair e1 e2) =
+  lem_fv_in_env_pair g e1 e2;
+  let t = mk_pair t1 t2 in
+  introduce forall b (s:gsub g b) fs_s. s ∽ fs_s ==>  t ⦂ ((fs_e1 fs_s, fs_e2 fs_s), gsubst s (EPair e1 e2)) with begin
+    let fs_e1 = fs_e1 fs_s in
+    let fs_e2 = fs_e2 fs_s in
+    let fs_e = (fs_e1, fs_e2) in
+    let e = EPair (gsubst s e1) (gsubst s e2) in
+    assert (gsubst s (EPair e1 e2) == e);
+    let EPair e1 e2 = e in
+    introduce s ∽ fs_s ==>  t ⦂ (fs_e, e) with _. begin
+      introduce forall (e':closed_exp). steps e e' /\ irred e' ==> t ∋ (fs_e, e') with begin
+        introduce _ ==> t ∋ (fs_e, e') with h. begin
+          let steps_e_e' : squash (steps e e') = () in
+          FStar.Squash.map_squash #_ #(squash (t ∋ (fs_e, e'))) steps_e_e' (fun steps_e_e' ->
+            let (e1', e2') = destruct_steps_epair e1 e2 e' steps_e_e' in
+            assert (t1 ∋ (fs_e1, e1'));
+            assert (t2 ∋ (fs_e2, e2'));
+            assert (t ∋ (fs_e, EPair e1' e2'));
+            lem_values_are_expressions t fs_e (EPair e1' e2')
           )
         end
       end
